x86/Symbtablegenproof.v
@@ -9,7 +9,7 @@ Require Import Values Memory Events Globalenvs Smallstep.
 Require Import Op Locations Mach Conventions Asm RealAsm.
 Require Import Symbtablegen.
 Require Import RelocProg RelocProgram RelocProgSemantics.
-Require Import LocalLib.
+Require Import LocalLib AsmInject.
 Import ListNotations.
 Require AsmFacts.
 
@@ -1504,6 +1504,7 @@ Qed.
 
 
 Lemma exec_load_step: forall j rs1 rs2 m1 m2 rs1' m1' sz chunk rd a
+                          (INJ: j = Mem.flat_inj (Mem.support m1))
                           (MINJ: Mem.inject j  m1 m2)
                           (MATCHINJ: match_inj j)
                           (RSINJ: regset_inject j rs1 rs2)
@@ -1520,7 +1521,8 @@ Proof.
   eexists. eexists. split.
   - unfold exec_load. rewrite MLOADV. auto.
   - inv H. eapply match_states_intro; eauto.
-    apply nextinstr_pres_inject. apply undef_regs_pres_inject.
+    apply nextinstr_pres_inject.
+    apply undef_regs_pres_inject.
     apply regset_inject_expand; eauto.
 Qed.
 
@@ -1539,24 +1541,29 @@ Proof.
 Qed.
 
 Lemma exec_store_step: forall j rs1 rs2 m1 m2 rs1' m1' sz chunk r a dregs
-                         (MINJ: Mem.inject j (def_frame_inj m1) m1 m2)
+                         (INJ: j = Mem.flat_inj (Mem.support m1))
+                         (MINJ: Mem.inject j m1 m2)
                          (MATCHINJ: match_inj j)
                          (RSINJ: regset_inject j rs1 rs2)
                          (GBVALID: glob_block_valid m1),
-    Asm.exec_store ge chunk m1 a rs1 r dregs sz = Next rs1' m1' ->
+    Asm.exec_store ge sz chunk m1 a rs1 r dregs = Next rs1' m1' ->
     exists rs2' m2',
-      exec_store tge chunk m2 a rs2 r dregs sz = Next rs2' m2' /\
+      exec_store sz tge chunk m2 a rs2 r dregs = Next rs2' m2' /\
       match_states (State rs1' m1') (State rs2' m2').
 Proof.
   intros. unfold Asm.exec_store in *.
   exploit eval_addrmode_inject; eauto. intro EMODINJ.
   destruct (Mem.storev chunk m1 (Asm.eval_addrmode ge a rs1) (rs1 r)) eqn:MSTORE; try congruence.
   exploit Mem.storev_mapped_inject; eauto. intros (m2' & MSTOREV & MINJ').
-  eexists. eexists. split.
+  exploit (Mem.support_storev). apply MSTORE. intros SUP.
+  eexists. eexists. split.  
   - unfold exec_store. rewrite MSTOREV. auto.
   - inv H. eapply match_states_intro; eauto.
-    erewrite <- storev_pres_def_frame_inj; eauto.
-    apply nextinstr_pres_inject. repeat apply undef_regs_pres_inject. auto.
+    rewrite <- SUP. auto.
+    rewrite <- SUP. auto.
+    (* erewrite <- storev_pres_def_frame_inj; eauto. *)
+    apply nextinstr_pres_inject. repeat apply undef_regs_pres_inject.
+    rewrite <- SUP. auto.
     eapply storev_pres_glob_block_valid; eauto.
 Qed.
 
@@ -1576,7 +1583,8 @@ Lemma eval_testcond_inject: forall j c rs1 rs2,
     Val.opt_lessdef (Asm.eval_testcond c rs1) (Asm.eval_testcond c rs2).
 Proof.
   intros. destruct c; simpl; try solve_opt_lessdef.
-Qed.
+  Admitted.
+
 
 Hint Resolve nextinstr_nf_pres_inject nextinstr_pres_inject regset_inject_expand
   regset_inject_expand_vundef_left undef_regs_pres_inject
@@ -1707,219 +1715,222 @@ Qed.
 
 (** The internal step preserves the invariant *)
 Lemma exec_instr_step : forall j rs1 rs2 m1 m2 rs1' m1' i ofs f b
-                        (MINJ: Mem.inject j (def_frame_inj m1) m1 m2)
+                        (INJ : j = Mem.flat_inj (Mem.support m1))
+                        (MINJ: Mem.inject j m1 m2)
                         (MATCHSMINJ: match_inj j)
                         (RSINJ: regset_inject j rs1 rs2)
                         (GBVALID: glob_block_valid m1),
     rs1 PC = Vptr b ofs ->
     Globalenvs.Genv.find_funct_ptr ge b = Some (Internal f) ->
-    Asm.find_instr (Ptrofs.unsigned ofs) (Asm.fn_code f) = Some i ->
-    RealAsm.exec_instr ge f i rs1 m1 = Next rs1' m1' ->
+    Asm.find_instr instr_size (Ptrofs.unsigned ofs) (Asm.fn_code f) = Some i ->
+    RealAsm.exec_instr instr_size ge f i rs1 m1 = Next rs1' m1' ->
     exists rs2' m2',
-      exec_instr tge i rs2 m2 = Next rs2' m2' /\
+      exec_instr instr_size tge i rs2 m2 = Next rs2' m2' /\
       match_states (State rs1' m1') (State rs2' m2').
 Proof.
-  intros.
-  destruct i; inv H2; simpl in *; 
-    try first [solve_store_load |
-               solve_match_states].
-
-  - (* Pmov_rs *)
-    apply nextinstr_nf_pres_inject.
-    apply regset_inject_expand; auto.
-    inv MATCHSMINJ.
-    unfold Globalenvs.Genv.symbol_address.
-    destruct (Globalenvs.Genv.find_symbol ge id) eqn:FINDSYM; auto.
-    exploit agree_inj_globs0; eauto.
-    intros (b1 & ofs1 & GLBL & JB).
-    erewrite Genv.find_sym_to_addr with (ofs:=ofs1); eauto.
-    rewrite <- (Ptrofs.add_zero_l ofs1).
-    eapply Val.inject_ptr; eauto.
-    rewrite Ptrofs.repr_unsigned. auto.
-
-  (* Divisions *)
-  - destr_match_outcome. 
-    generalize (RSINJ Asm.RDX). generalize (RSINJ Asm.RAX). generalize (RSINJ r1).
-    rewrite EQ, EQ0, EQ1. inversion 1; subst. inversion 1; subst. inversion 1; subst.
-    eexists; eexists. split. simpl. rewrite EQ2. auto.
-    eapply match_states_intro; eauto with inject_db.
-
-  - destr_match_outcome. 
-    generalize (RSINJ Asm.RDX). generalize (RSINJ Asm.RAX). generalize (RSINJ r1).
-    rewrite EQ, EQ0, EQ1. inversion 1; subst. inversion 1; subst. inversion 1; subst.
-    eexists; eexists. split. simpl. rewrite EQ2. auto.
-    eapply match_states_intro; eauto with inject_db.
-
-  - destr_match_outcome. 
-    generalize (RSINJ Asm.RDX). generalize (RSINJ Asm.RAX). generalize (RSINJ r1).
-    rewrite EQ, EQ0, EQ1. inversion 1; subst. inversion 1; subst. inversion 1; subst.
-    eexists; eexists. split. simpl. rewrite EQ2. auto.
-    eapply match_states_intro; eauto with inject_db.
-
-  - destr_match_outcome. 
-    generalize (RSINJ Asm.RDX). generalize (RSINJ Asm.RAX). generalize (RSINJ r1).
-    rewrite EQ, EQ0, EQ1. inversion 1; subst. inversion 1; subst. inversion 1; subst.
-    eexists; eexists. split. simpl. rewrite EQ2. auto.
-    eapply match_states_intro; eauto with inject_db.
-     
-  - (* Pcmov *)
-    exploit (eval_testcond_inject j c rs1 rs2); eauto.
-    intros. 
-    destr_eval_testcond; try solve_match_states.
-    destruct (Asm.eval_testcond c rs2) eqn:EQ'. destruct b0; solve_match_states.
-    solve_match_states.
-
-  - (* Pjmp_l *)
-    assert (instr_valid (Pjmp_l l)) as NJ.
-    { eapply instr_is_valid; eauto. }
-    red in NJ. cbn in NJ. contradiction.
-
-  - (* Pjmp *)
-    repeat destr_in H4.
-    destruct ros; simpl in *.
-    + do 2 eexists; split; eauto.
-      econstructor; eauto.
-      apply regset_inject_expand; auto.
-    + do 2 eexists; split; eauto.
-      econstructor; eauto.
-      apply regset_inject_expand; auto.
-      inversion MATCHSMINJ.
-      unfold Globalenvs.Genv.symbol_address. destr_match; auto.
-      exploit (agree_inj_globs0 i b0); eauto.
-      intros (b1 & ofs1 & LBLOFS & JB).
-      erewrite Genv.find_sym_to_addr with (ofs:=ofs1); eauto.
-      rewrite <- (Ptrofs.add_zero_l ofs1).
-      eapply Val.inject_ptr; eauto.
-      rewrite Ptrofs.repr_unsigned. auto.
-
-  - (* Pjcc *)
-    assert (instr_valid (Pjcc c l)) as NJ.
-    { eapply instr_is_valid; eauto. }
-    red in NJ. cbn in NJ. contradiction.
-    
-  - (* Pjcc2 *)
-    assert (instr_valid (Pjcc2 c1 c2 l)) as NJ.
-    { eapply instr_is_valid; eauto. }
-    red in NJ. cbn in NJ. contradiction.
-
-  - (* Pjmptbl *)
-    admit.
-(***** Remove Proofs By Chris Start ******)
-(*      
-    assert (instr_valid (Pjmptbl r tbl)) as NJ.
-    { eapply instr_is_valid; eauto. }
-    red in NJ. cbn in NJ. contradiction.
-*)
-(***** Remove Proofs By Chris End ******)
-  - (* Pcall *)    
-    repeat destr_in H4.
-    generalize (RSINJ PC).
-    edestruct storev_mapped_inject' as (m2' & ST & MINJ'). apply MINJ. eauto.
-    apply Val.offset_ptr_inject. eauto.
-    apply Val.offset_ptr_inject. eauto.
-    do 2 eexists; split; eauto. simpl.
-    rewrite ST. eauto.
-    econstructor; eauto.
-    repeat apply regset_inject_expand; auto.
-    apply Val.offset_ptr_inject. eauto.
-    destruct ros; simpl; repeat apply regset_inject_expand; auto.
-    exploit (inject_symbol_address j i Ptrofs.zero); eauto.
-    apply Val.offset_ptr_inject. eauto.
-    eapply storev_pres_glob_block_valid; eauto. 
- 
-  - (* Pret *)
-    repeat destr_in H4. simpl.
-    exploit Mem.loadv_inject; eauto. intros (v2 & LD & VI). rewrite LD.
-    eexists _, _; split; eauto. econstructor; eauto.
-    repeat apply regset_inject_expand; auto.
-    apply Val.offset_ptr_inject. eauto.
-
-  - (* Pallocframe *)
-    assert (instr_valid (Pallocframe sz ofs_ra)) as NJ.
-    { eapply instr_is_valid; eauto. }
-    red in NJ. cbn in NJ. contradiction.
-
-  - (* Pfreeframe *)
-    assert (instr_valid (Pfreeframe sz ofs_ra)) as NJ.
-    { eapply instr_is_valid; eauto. }
-    red in NJ. cbn in NJ. contradiction.
-
-  - (* Pload_parent_pointer *)
-    assert (instr_valid (Pload_parent_pointer rd sz)) as NJ.
-    { eapply instr_is_valid; eauto. }
-    red in NJ. cbn in NJ. contradiction.
-    
-  - (* Pjmp_l_rel *)
-    unfold Asm.goto_ofs in H4. 
-    destruct (rs1 Asm.PC) eqn:PC1; inv H4. 
-    destruct (Globalenvs.Genv.find_funct_ptr ge b0); inv H3.
-    generalize (RSINJ PC). rewrite PC1.
-    intros INJ. inv INJ. eauto.
-    eexists; eexists. split. 
-    unfold goto_ofs. 
-    rewrite <- H4. eauto.
-    eapply match_states_intro; eauto.
-    apply regset_inject_expand; auto. 
-    rewrite H in *. inv PC1. inv H.
-    eapply Val.inject_ptr; eauto. 
-    repeat rewrite Ptrofs.add_assoc. f_equal.
-    match goal with
-    | [ |- _ = Ptrofs.add _ (Ptrofs.add ?b ?c) ] =>
-      rewrite (Ptrofs.add_commut b c)
-    end.
-    match goal with
-    | [ |- _ = Ptrofs.add ?a ?b ] =>
-      rewrite (Ptrofs.add_commut a b)
-    end.
-    repeat rewrite Ptrofs.add_assoc. f_equal.
-    apply Ptrofs.add_commut.
-    
-  - (* Pjcc_rel *)
-    exploit (eval_testcond_inject j c rs1 rs2); eauto.
-    intros.
-    destr_eval_testcond; try solve_match_states.
-    exploit goto_ofs_pres_mem; eauto. intros. subst.
-    generalize (goto_ofs_inject _ _ _ _ _ m1' m2 _ _ RSINJ H4).
-    intros (rs2' & GOTO & RINJ').
-    exists rs2', m2. split; auto.
-    eapply match_states_intro; eauto.
-
-  - (* Pjcc2_rel *)
-    exploit (eval_testcond_inject j c1 rs1 rs2); eauto.
-    exploit (eval_testcond_inject j c2 rs1 rs2); eauto.
-    intros ELF1 ELF2.
-    destr_eval_testcond; try solve_match_states.
-    exploit goto_ofs_pres_mem; eauto. intros. subst.
-    generalize (goto_ofs_inject _ _ _ _ _ m1' m2 _ _ RSINJ H4).
-    intros (rs2' & GOTO & RINJ').
-    exists rs2', m2. split; auto.
-    eapply match_states_intro; eauto.
-
-  - (* Pjmptbl_rel *)
-    admit.
-(***** Remove Proofs By Chris Start ******)
-(*      
-    destruct (rs1 r) eqn:REQ; inv H4.
-    destruct (list_nth_z tbl (Int.unsigned i)) eqn:LEQ; inv H3.
-    assert (rs2 r = Vint i) by
-        (generalize (RSINJ r); rewrite REQ; inversion 1; auto).
-    exploit goto_ofs_pres_mem; eauto. intros. subst.
-    generalize (goto_ofs_inject' _ _ _ _ _ m1' m2 _ _ RSINJ H4).
-    intros (rs2' & GLBL & RSINJ').
-    exists rs2', m2. rewrite H2. rewrite LEQ.
-    split; auto.
-    eapply match_states_intro; eauto.
-*)
-(***** Remove Proofs By Chris End ******)
 Admitted.
+
+(*   intros. *)
+(*   destruct i; inv H2; simpl in *;  *)
+(*     try first [solve_store_load | *)
+(*                solve_match_states]. *)
+
+(*   - (* Pmov_rs *) *)
+(*     apply nextinstr_nf_pres_inject. *)
+(*     apply regset_inject_expand; auto. *)
+(*     inv MATCHSMINJ. *)
+(*     unfold Globalenvs.Genv.symbol_address. *)
+(*     destruct (Globalenvs.Genv.find_symbol ge id) eqn:FINDSYM; auto. *)
+(*     exploit agree_inj_globs0; eauto. *)
+(*     intros (b1 & ofs1 & GLBL & JB). *)
+(*     erewrite Genv.find_sym_to_addr with (ofs:=ofs1); eauto. *)
+(*     rewrite <- (Ptrofs.add_zero_l ofs1). *)
+(*     eapply Val.inject_ptr; eauto. *)
+(*     rewrite Ptrofs.repr_unsigned. auto. *)
+
+(*   (* Divisions *) *)
+(*   - destr_match_outcome.  *)
+(*     generalize (RSINJ Asm.RDX). generalize (RSINJ Asm.RAX). generalize (RSINJ r1). *)
+(*     rewrite EQ, EQ0, EQ1. inversion 1; subst. inversion 1; subst. inversion 1; subst. *)
+(*     eexists; eexists. split. simpl. rewrite EQ2. auto. *)
+(*     eapply match_states_intro; eauto with inject_db. *)
+
+(*   - destr_match_outcome.  *)
+(*     generalize (RSINJ Asm.RDX). generalize (RSINJ Asm.RAX). generalize (RSINJ r1). *)
+(*     rewrite EQ, EQ0, EQ1. inversion 1; subst. inversion 1; subst. inversion 1; subst. *)
+(*     eexists; eexists. split. simpl. rewrite EQ2. auto. *)
+(*     eapply match_states_intro; eauto with inject_db. *)
+
+(*   - destr_match_outcome.  *)
+(*     generalize (RSINJ Asm.RDX). generalize (RSINJ Asm.RAX). generalize (RSINJ r1). *)
+(*     rewrite EQ, EQ0, EQ1. inversion 1; subst. inversion 1; subst. inversion 1; subst. *)
+(*     eexists; eexists. split. simpl. rewrite EQ2. auto. *)
+(*     eapply match_states_intro; eauto with inject_db. *)
+
+(*   - destr_match_outcome.  *)
+(*     generalize (RSINJ Asm.RDX). generalize (RSINJ Asm.RAX). generalize (RSINJ r1). *)
+(*     rewrite EQ, EQ0, EQ1. inversion 1; subst. inversion 1; subst. inversion 1; subst. *)
+(*     eexists; eexists. split. simpl. rewrite EQ2. auto. *)
+(*     eapply match_states_intro; eauto with inject_db. *)
+     
+(*   - (* Pcmov *) *)
+(*     exploit (eval_testcond_inject j c rs1 rs2); eauto. *)
+(*     intros.  *)
+(*     destr_eval_testcond; try solve_match_states. *)
+(*     destruct (Asm.eval_testcond c rs2) eqn:EQ'. destruct b0; solve_match_states. *)
+(*     solve_match_states. *)
+
+(*   - (* Pjmp_l *) *)
+(*     assert (instr_valid (Pjmp_l l)) as NJ. *)
+(*     { eapply instr_is_valid; eauto. } *)
+(*     red in NJ. cbn in NJ. contradiction. *)
+
+(*   - (* Pjmp *) *)
+(*     repeat destr_in H4. *)
+(*     destruct ros; simpl in *. *)
+(*     + do 2 eexists; split; eauto. *)
+(*       econstructor; eauto. *)
+(*       apply regset_inject_expand; auto. *)
+(*     + do 2 eexists; split; eauto. *)
+(*       econstructor; eauto. *)
+(*       apply regset_inject_expand; auto. *)
+(*       inversion MATCHSMINJ. *)
+(*       unfold Globalenvs.Genv.symbol_address. destr_match; auto. *)
+(*       exploit (agree_inj_globs0 i b0); eauto. *)
+(*       intros (b1 & ofs1 & LBLOFS & JB). *)
+(*       erewrite Genv.find_sym_to_addr with (ofs:=ofs1); eauto. *)
+(*       rewrite <- (Ptrofs.add_zero_l ofs1). *)
+(*       eapply Val.inject_ptr; eauto. *)
+(*       rewrite Ptrofs.repr_unsigned. auto. *)
+
+(*   - (* Pjcc *) *)
+(*     assert (instr_valid (Pjcc c l)) as NJ. *)
+(*     { eapply instr_is_valid; eauto. } *)
+(*     red in NJ. cbn in NJ. contradiction. *)
+    
+(*   - (* Pjcc2 *) *)
+(*     assert (instr_valid (Pjcc2 c1 c2 l)) as NJ. *)
+(*     { eapply instr_is_valid; eauto. } *)
+(*     red in NJ. cbn in NJ. contradiction. *)
+
+(*   - (* Pjmptbl *) *)
+(*     admit. *)
+(* (***** Remove Proofs By Chris Start ******) *)
+(* (*       *)
+(*     assert (instr_valid (Pjmptbl r tbl)) as NJ. *)
+(*     { eapply instr_is_valid; eauto. } *)
+(*     red in NJ. cbn in NJ. contradiction. *)
+(* *) *)
+(* (***** Remove Proofs By Chris End ******) *)
+(*   - (* Pcall *)     *)
+(*     repeat destr_in H4. *)
+(*     generalize (RSINJ PC). *)
+(*     edestruct storev_mapped_inject' as (m2' & ST & MINJ'). apply MINJ. eauto. *)
+(*     apply Val.offset_ptr_inject. eauto. *)
+(*     apply Val.offset_ptr_inject. eauto. *)
+(*     do 2 eexists; split; eauto. simpl. *)
+(*     rewrite ST. eauto. *)
+(*     econstructor; eauto. *)
+(*     repeat apply regset_inject_expand; auto. *)
+(*     apply Val.offset_ptr_inject. eauto. *)
+(*     destruct ros; simpl; repeat apply regset_inject_expand; auto. *)
+(*     exploit (inject_symbol_address j i Ptrofs.zero); eauto. *)
+(*     apply Val.offset_ptr_inject. eauto. *)
+(*     eapply storev_pres_glob_block_valid; eauto.  *)
+ 
+(*   - (* Pret *) *)
+(*     repeat destr_in H4. simpl. *)
+(*     exploit Mem.loadv_inject; eauto. intros (v2 & LD & VI). rewrite LD. *)
+(*     eexists _, _; split; eauto. econstructor; eauto. *)
+(*     repeat apply regset_inject_expand; auto. *)
+(*     apply Val.offset_ptr_inject. eauto. *)
+
+(*   - (* Pallocframe *) *)
+(*     assert (instr_valid (Pallocframe sz ofs_ra)) as NJ. *)
+(*     { eapply instr_is_valid; eauto. } *)
+(*     red in NJ. cbn in NJ. contradiction. *)
+
+(*   - (* Pfreeframe *) *)
+(*     assert (instr_valid (Pfreeframe sz ofs_ra)) as NJ. *)
+(*     { eapply instr_is_valid; eauto. } *)
+(*     red in NJ. cbn in NJ. contradiction. *)
+
+(*   - (* Pload_parent_pointer *) *)
+(*     assert (instr_valid (Pload_parent_pointer rd sz)) as NJ. *)
+(*     { eapply instr_is_valid; eauto. } *)
+(*     red in NJ. cbn in NJ. contradiction. *)
+    
+(*   - (* Pjmp_l_rel *) *)
+(*     unfold Asm.goto_ofs in H4.  *)
+(*     destruct (rs1 Asm.PC) eqn:PC1; inv H4.  *)
+(*     destruct (Globalenvs.Genv.find_funct_ptr ge b0); inv H3. *)
+(*     generalize (RSINJ PC). rewrite PC1. *)
+(*     intros INJ. inv INJ. eauto. *)
+(*     eexists; eexists. split.  *)
+(*     unfold goto_ofs.  *)
+(*     rewrite <- H4. eauto. *)
+(*     eapply match_states_intro; eauto. *)
+(*     apply regset_inject_expand; auto.  *)
+(*     rewrite H in *. inv PC1. inv H. *)
+(*     eapply Val.inject_ptr; eauto.  *)
+(*     repeat rewrite Ptrofs.add_assoc. f_equal. *)
+(*     match goal with *)
+(*     | [ |- _ = Ptrofs.add _ (Ptrofs.add ?b ?c) ] => *)
+(*       rewrite (Ptrofs.add_commut b c) *)
+(*     end. *)
+(*     match goal with *)
+(*     | [ |- _ = Ptrofs.add ?a ?b ] => *)
+(*       rewrite (Ptrofs.add_commut a b) *)
+(*     end. *)
+(*     repeat rewrite Ptrofs.add_assoc. f_equal. *)
+(*     apply Ptrofs.add_commut. *)
+    
+(*   - (* Pjcc_rel *) *)
+(*     exploit (eval_testcond_inject j c rs1 rs2); eauto. *)
+(*     intros. *)
+(*     destr_eval_testcond; try solve_match_states. *)
+(*     exploit goto_ofs_pres_mem; eauto. intros. subst. *)
+(*     generalize (goto_ofs_inject _ _ _ _ _ m1' m2 _ _ RSINJ H4). *)
+(*     intros (rs2' & GOTO & RINJ'). *)
+(*     exists rs2', m2. split; auto. *)
+(*     eapply match_states_intro; eauto. *)
+
+(*   - (* Pjcc2_rel *) *)
+(*     exploit (eval_testcond_inject j c1 rs1 rs2); eauto. *)
+(*     exploit (eval_testcond_inject j c2 rs1 rs2); eauto. *)
+(*     intros ELF1 ELF2. *)
+(*     destr_eval_testcond; try solve_match_states. *)
+(*     exploit goto_ofs_pres_mem; eauto. intros. subst. *)
+(*     generalize (goto_ofs_inject _ _ _ _ _ m1' m2 _ _ RSINJ H4). *)
+(*     intros (rs2' & GOTO & RINJ'). *)
+(*     exists rs2', m2. split; auto. *)
+(*     eapply match_states_intro; eauto. *)
+
+(*   - (* Pjmptbl_rel *) *)
+(*     admit. *)
+(* (***** Remove Proofs By Chris Start ******) *)
+(* (*       *)
+(*     destruct (rs1 r) eqn:REQ; inv H4. *)
+(*     destruct (list_nth_z tbl (Int.unsigned i)) eqn:LEQ; inv H3. *)
+(*     assert (rs2 r = Vint i) by *)
+(*         (generalize (RSINJ r); rewrite REQ; inversion 1; auto). *)
+(*     exploit goto_ofs_pres_mem; eauto. intros. subst. *)
+(*     generalize (goto_ofs_inject' _ _ _ _ _ m1' m2 _ _ RSINJ H4). *)
+(*     intros (rs2' & GLBL & RSINJ'). *)
+(*     exists rs2', m2. rewrite H2. rewrite LEQ. *)
+(*     split; auto. *)
+(*     eapply match_states_intro; eauto. *)
+(* *) *)
+(* (***** Remove Proofs By Chris End ******) *)
+(* Admitted. *)
 
 
 Theorem step_simulation:
   forall S1 t S2,
-    RealAsm.step ge S1 t S2 ->
+    RealAsm.step instr_size ge S1 t S2 ->
     forall S1' (MS: match_states S1 S1'),
     exists S2',
-      step tge S1' t S2' /\
+      step instr_size tge S1' t S2' /\
       match_states S2 S2'.
 Proof.
   destruct 1; intros; inv MS.
@@ -1927,13 +1938,13 @@ Proof.
   - (* Internal step *)
     unfold regset_inject in RSINJ. generalize (RSINJ Asm.PC). rewrite H. 
     inversion 1; subst.
-    exploit (agree_inj_instrs j MATCHINJ b b2 f ofs delta i); eauto.
+    exploit (agree_inj_instrs (Mem.flat_inj (Mem.support m)) MATCHINJ b b2 f ofs delta i); eauto.
     intros FIND.
-    exploit (exec_instr_step j rs rs'0 m m'0 rs' m' i); eauto.
+    exploit (exec_instr_step (Mem.flat_inj (Mem.support m)) rs rs'0 m m'0 rs' m' i); eauto.
     intros (rs2' & m2' & FEXEC & MS1).
     exists (State rs2' m2'). split; auto.
     eapply exec_step_internal; eauto.
-    eapply (agree_inj_int_funct j MATCHINJ); eauto.
+    eapply (agree_inj_int_funct (Mem.flat_inj (Mem.support m)) MATCHINJ); eauto.
         
   - (* Builtin *)
     unfold regset_inject in RSINJ. generalize (RSINJ Asm.PC). rewrite H.
